\documentclass{report}

\input{~/dev/latex/template/preamble.tex}
\input{~/dev/latex/template/macros.tex}

\title{\Huge{}}
\author{\huge{Nathan Warner}}
\date{\huge{}}
\pagestyle{fancy}
\fancyhf{}
\lhead{Warner \thepage}
\rhead{}
% \lhead{\leftmark}
\cfoot{\thepage}
% \setborder
% \usepackage[default]{sourcecodepro}
% \usepackage[T1]{fontenc}

\begin{document}
    % \maketitle
    % \tableofcontents
    \pagebreak \bigbreak \noindent
    Nate Warner \ \quad \quad \quad \quad \quad \quad \quad \quad \quad \quad \quad \quad \quad \quad \quad \quad \quad  MATH 230 \quad  \quad \quad \quad \quad \quad \quad \quad \quad \ \ \quad \quad August 5, 2023
    \begin{center}
        \textbf{Homework/Worksheet 5 - Due: Wednesday, October 11}
    \end{center}
    \bigbreak \noindent 
    \begin{mdframed}
        \textbf{1. Evaluate the following integrals using the method of integration by parts:}
        \begin{enumerate}[label=(\alph*)]
            \item $\int x e^{4 x} d x$
            \item $\int \ln x d x$
            \item $\int x^4 \ln x d x$
            \item $\int x \cos 3 x d x$
            \item $\int e^{2 x} \sin (5 x) d x$
            \item $\int_0^1 e^{\sqrt{x}} d x$
        \end{enumerate}
    \end{mdframed}

    \bigbreak \noindent 
    \textbf{1.a}
    \bigbreak \noindent 
    \begin{minipage}[t]{0.47\textwidth}
    \begin{align*}
        &u = x \quad dv = e^{4x}\ dx \\
        &du = dx \quad v = \frac{1}{4}e^{4x}
    .\end{align*}    
    \end{minipage}
    \begin{minipage}[t]{0.47\textwidth}
    \begin{align*}
        &\int xe^{4x}\ dx \\
        &=\frac{1}{4}xe^{4x} - \int \frac{1}{4}e^{4x}\ dx \\
        &= \frac{1}{4}xe^{4x} - \frac{1}{16}e^{4x} + C
    .\end{align*}
    \end{minipage}

    \bigbreak \noindent 
    \textbf{1.b}
    \bigbreak \noindent 
    \begin{minipage}[t]{0.47\textwidth}
        \begin{align*}
            &u = \ln{x} \quad dv = dx \\
            &du = \frac{1}{x}\ dx \quad v = x
        .\end{align*}
    \end{minipage}
    \begin{minipage}[t]{0.47\textwidth}
        \begin{align*}
            &\int \ln{x}\ dx \\
           &=x\ln{x} - \int x \cdot \frac{1}{x}\ dx \\
           &= x\ln{x} - x + C
        .\end{align*}
    \end{minipage}

    \bigbreak \noindent 
    \textbf{1.c}
    \bigbreak \noindent 
    \begin{minipage}[t]{0.47\textwidth}
        \begin{align*}
            &u = \ln{x} \quad dv = x^{4}\ dx \\
            &du = \frac{1}{x}\ dx \quad v = \frac{1}{5}x^{5}
        .\end{align*}
    \end{minipage}
    \begin{minipage}[t]{0.47\textwidth}
        \begin{align*}
           &\int x^{4}\ln{x}\ dx \\ 
           &=\frac{1}{5}x^{5}\ln{x} - \int \frac{1}{5}x^{5} \cdot \frac{1}{x}\ dx \\
           &=\frac{1}{5}x^{5}\ln{x} - \int \frac{1}{5}x^{4}\ dx \\
           &= \frac{1}{5}x^{5}\ln{x} - \frac{1}{25}x^{5} + C
        .\end{align*}
    \end{minipage}

    \pagebreak \bigbreak \noindent 
    \textbf{1.d}
    \bigbreak \noindent 
    \begin{minipage}[t]{0.47\textwidth}
        \begin{align*}
            &u = x \quad dv = \cos{3x}\ dx \\
            &du = dx \quad v = \frac{1}{3}\sin{3x}
        .\end{align*}
    \end{minipage}
    \begin{minipage}[t]{0.47\textwidth}
        \begin{align*}
            &\int x\cos{3x}\ dx \\
            &=\frac{1}{3}x\sin{3x} - \int \frac{1}{3}\sin{3x}\ dx \\
            &= \frac{1}{3}x\sin{3x} + \frac{1}{9}\cos{3x} + C
        .\end{align*}
    \end{minipage}

    \bigbreak \noindent 
    \textbf{1.e}
    \bigbreak \noindent 
    \begin{minipage}[t]{0.47\textwidth}
        \begin{align*}
            &u = \sin{5x} \quad dv = e^{2x}\ dx \\
            &du = 5\cos{5x}\ dx \quad v = \frac{1}{2}e^{2x}
        .\end{align*}
    \end{minipage}
    \begin{minipage}[t]{0.47\textwidth}
        \begin{align*}
            &\int e^{2x}\sin{5x}\ dx \\
            &=\frac{1}{2}e^{2x}\sin{5x} - \int \frac{5}{2}e^{2x}\cos{5x}\ dx \\
            &=\frac{1}{2}e^{2x}\sin{5x} - \frac{5}{2}\int e^{2x}\cos{5x}\ dx
        .\end{align*}
    \end{minipage}
    \bigbreak \noindent 
    \begin{minipage}[t]{0.47\textwidth}
        \begin{align*}
            &u = \cos{5x} \quad dv = e^{2x}\ dx \\
            &du = -5\sin{5x}\ dx \quad v = \frac{1}{2}e^{2x}
        .\end{align*}
    \end{minipage}
    \begin{minipage}[t]{0.47\textwidth}
        \begin{align*}
            &\int e^{2x}\cos{5x}\ dx \\
            &=\frac{1}{2}e^{2x}\cos{5x} - \int -\frac{5}{2}e^{2x}\sin{5x}\ dx \\
            &=\frac{1}{2}e^{2x}\cos{5x} + \frac{5}{2}\int e^{2x}\sin{5x}\ dx \\
        .\end{align*}
    \end{minipage}
    \bigbreak \noindent 
    Thus we have:
    \begin{align*}
        &\int e^{2x}\sin{5x}\ dx = \frac{1}{2}e^{2x}\sin{5x} - \frac{5}{2}\left[\frac{1}{2}e^{2x}\cos{5x}+\frac{5}{2}\int e^{2x}\sin{5x}\ dx\right] \\
        &=\frac{1}{2}e^{2x}\sin{5x} -\frac{5}{4}e^{2x}\cos{5x} - \frac{25}{4}\int e^{2x}\sin{5x}\ dx
    .\end{align*}
    \bigbreak \noindent 
    Let $I = \int e^{2x}\sin{5x}\ dx$
    \begin{align*}
        &\left(\frac{25}{4} +1\right) I = \frac{1}{2}e^{2x}\sin{5x} -\frac{5}{4}e^{2x}\cos{5x} \\
        &I = \frac{4}{29}\left(\frac{1}{2}e^{2x}\sin{5x} -\frac{5}{4}e^{2x}\cos{5x}\right) \\
        &\int e^{2x}\sin{5x}\ dx = \frac{4}{29}\left(\frac{1}{2}e^{2x}\sin{5x} -\frac{5}{4}e^{2x}\cos{5x}\right)  + C\\
    .\end{align*}

    \pagebreak \bigbreak \noindent 
    \textbf{1.f}
    \bigbreak \noindent 
    \begin{minipage}[t]{0.47\textwidth}
        \begin{align*}
            &\text{Let $u=x^{\frac{1}{2}}$} \\
            &du= \frac{1}{2x^{\frac{1}{2}}}dx \\
            &2x^{\frac{1}{2}}du = dx \\
            &u(a) = 0 \\
            &u(b) = 1
        .\end{align*}    
    \end{minipage}
    \begin{minipage}[t]{0.47\textwidth}
        \begin{align*}
            &\int_{0}^{1}\ e^{x^{\frac{1}{2}}}\ dx \\
            &=2\int_{0}^{1}\ ue^{u}\ du 
        .\end{align*}
    \end{minipage}
    \bigbreak \noindent 
    \begin{minipage}[t]{0.47\textwidth}
        \begin{align*}
            w = u \quad dv = e^{u} \\
            dw = du \quad v = e^{u}
        .\end{align*}
    \end{minipage}
    \begin{minipage}[t]{0.47\textwidth}
        \begin{align*}
            &2\left(ue^{u} - \int e^{u}\ du\right) \\
            &=2\left(ue^{u} - e^{u}\right) + C \\
            &=2\left(x^{\frac{1}{2}}e^{x^{\frac{1}{2}}} - e^{x^{\frac{1}{2}}}\right) + C \\
            &=2x^{\frac{1}{2}}e^{x^{\frac{1}{2}}} - 2e^{x^{\frac{1}{2}}} + C
        .\end{align*}
    \end{minipage}


    \pagebreak \bigbreak \noindent 
    \begin{mdframed}
        \textbf{2. Evaluate the following trigonometric integrals:}
        \begin{enumerate}[label=(\alph*)]
            \item $\int \sin ^7(2 x) \cos (2 x) d x$
            \item $\int \sin ^3 x \cos ^3 x d x$
            \item $\int \sin ^3 x d x$
            \item $\int \tan ^2 x \sec x d x$
            \item $\int \cos ^5 x d x$
            \item $\int_0^\pi \sin 3 x \cos 5 x d x$
        \end{enumerate}

    \end{mdframed}

        \bigbreak \noindent 
    \textbf{2.a}
    \bigbreak \noindent 
    \begin{minipage}[t]{0.47\textwidth}
        \begin{align*}
            &\text{Let $u=\sin{2x}$} \\
            &du = 2\cos{2x}\ dx \\
            &\frac{1}{2}du = \cos{2x}\ dx
        .\end{align*}
    \end{minipage}
    \begin{minipage}[t]{0.47\textwidth}
        \begin{align*}
            &\int \sin^{7}{2x}\cos{2x}\ dx \\
            &=\frac{1}{2}\int u^{7}\ du \\
            &= \frac{1}{2}\left(\frac{1}{8}u^{8}\right) + C \\
            &= \frac{1}{16}\sin^{8}{(2x)} + C
        .\end{align*}
    \end{minipage}

    \bigbreak \noindent 
    \textbf{2.b}
    \bigbreak \noindent 
    \begin{align*}
        &\int \sin^{3}{x}\cos^{3}{x}\ dx \\
        &=\int \sin^{3}{x}(1-\sin^{2}{x})\cos{x}\ dx
    .\end{align*}
    \bigbreak \noindent 
    \begin{minipage}[t]{0.47\textwidth}
        \begin{align*}
            &\text{Let $u=\sin{x}$} \\
            &du = \cos{x}\ dx
        .\end{align*}
    \end{minipage}
    \begin{minipage}[t]{0.47\textwidth}
        \begin{align*}
            &\int \sin^{3}{x}(1-\sin^{2}{x})\cos{x}\ dx \\
            &=\int u^{3}(1-u^{2})\ du \\
            &=\int u^{3} -u^{5}\ du \\
            &= \frac{1}{4}u^{4} - \frac{1}{6}u^{6} + C \\
            &= \frac{1}{4}\sin^{4}{x} - \frac{1}{6}\sin^{6}{x} + C
        .\end{align*}
    \end{minipage}

    \pagebreak  \bigbreak \noindent 
    \textbf{2.c}
    \bigbreak \noindent 
    By the reduction formula $\int \cos^{j}{x} = \frac{1}{j}\cos^{j-1}{x}\sin{x} + \frac{j-1}{j}\int \cos^{j-2}{x}\ dx $:
    \begin{align*}
        &\int \cos^{5}{x}\ dx \\
        &= \frac{1}{5}\cos^{4}{x}\sin{x} + \frac{4}{5}\int \cos^{3}{x}\ dx \\
        &= \frac{1}{5}\cos^{4}{x}\sin{x} + \frac{4}{5}\left[\frac{1}{3}\cos^{2}{x}\sin{x}+\frac{2}{3}\int \cos{x}\ dx\right] \\
        &= \frac{1}{5}\cos^{4}{x}\sin{x} + \frac{4}{15}\cos^{2}{x}\sin{x}+\frac{8}{15}\int \cos{x}\ dx \\
        &= \frac{1}{5}\cos^{4}{x}\sin{x} + \frac{4}{15}\cos^{2}{x}\sin{x}+\frac{8}{15}\sin{x} + C
    .\end{align*}

    \bigbreak \noindent 
    \textbf{2.d}
    \bigbreak \noindent 
    \begin{align*}
        &\int \sin^{3}{x}\cos^{3}{x}\ dx \\
        &=\int \sin^{3}{x}(1-\sin^{2}{x})\cos{x}\ dx \\
        &=\int u^{3}(1-u^{2})\ du \\
        &=\int u^{3} - u^{5}\ du \\
        &= \frac{1}{4}u^{4} -\frac{1}{6}u^{6} + C \\
        &=\frac{1}{4}\sin^{4}{x} - \frac{1}{6}\sin^{6}{x} + C 
    .\end{align*}

    \bigbreak \noindent 
    \textbf{2.e}
    \bigbreak \noindent 
    \begin{align*}
        &\int \tan^{2}{x}\sec{x}\ dx \\
        &=\int (\sec^{2}{x} -1)\sec{x}\ dx \\
        &= \int \sec^{3}{x} - \sec{x}\ dx \\
        &= \int \sec^{3}{x}\ dx - \int \sec{x}\ dx \\
        &I_{1} = \frac{1}{2}\sec^{2}{x}\sin{x} + \frac{1}{2}\int \sec{x}\ dx \quad \text{(By the reduction formula)} \\
        &= \frac{1}{2}\sec^{2}{x}\sin{x} + \frac{1}{2}\ln{\left(\abs{\sec{x} + \tan{x}}\right)} \\
        &I_{2} = \ln{\left(\abs{\sec{x} + \tan{x}}\right)} \\
        &\therefore \int \tan^{2}{x}\sec{x}\ dx = \frac{1}{2}\sec^{2}{x}\sin{x} + \frac{1}{2}\ln{\left(\abs{\sec{x} + \tan{x}}\right)}-\ln{(\abs{\sec{x} + \tan{x}})} + C \\
        &= \int \tan^{2}{x}\sec{x}\ dx = \frac{1}{2}\sec^{2}{x}\sin{x} - \frac{1}{2}\ln{\left(\abs{\sec{x} + \tan{x}}\right)} + C
    .\end{align*}

    \pagebreak \bigbreak \noindent 
    \textbf{2.f}
    \bigbreak \noindent 
    \begin{align*}
        &\int_0^{\pi} \sin{(3x)}\cos{(5x)}\ dx \\
        &=\int_0^{\pi}\frac{1}{2}\bigg[\sin{((3-5)x)} - \sin{((3+5)x)}\bigg]\ dx \\
        &=\frac{1}{2}\bigg[\int_0^{\pi} \sin{(-2x) - \sin{(8x)}}\ dx\bigg] \\
        &= \frac{1}{2}\bigg[\int_0^{\pi} \sin{(-2x)}\ dx -\int_0^{\pi}\sin{(8x)}\ dx\bigg] \\
        &= \frac{1}{2}\bigg[-\frac{1}{2}\int_{0}^{-2\pi}\ \sin{u}\ du - \frac{1}{8}\int_{0}^{8\pi}\ \sin{u}\ du\bigg] \\
        &=\frac{1}{2}\bigg[\frac{1}{2}\left(\cos{2\pi}-\cos{0}\right) +\frac{1}{8}(\cos{2\pi}-\cos{0}) \bigg] \\
        &= 0
    .\end{align*}





    
    

\end{document}
