\documentclass{report}

\input{~/dev/latex/template/preamble.tex}
\input{~/dev/latex/template/macros.tex}

\title{\Huge{}}
\author{\huge{Nathan Warner}}
\date{\huge{}}
\pagestyle{fancy}
\fancyhf{}
\lhead{Warner \thepage}
\rhead{}
% \lhead{\leftmark}
\cfoot{\thepage}
% \setborder
% \usepackage[default]{sourcecodepro}
% \usepackage[T1]{fontenc}

\begin{document}
    % \maketitle
    % \tableofcontents
    \pagebreak \bigbreak \noindent
    Nate Warner \ \quad \quad \quad \quad \quad \quad \quad \quad \quad \quad \quad \quad \quad \quad \quad \quad \quad  MATH 230 \quad  \quad \quad \quad \quad \quad \quad \quad \quad \ \ \quad \quad September 06, 2023
    \begin{center}
        \textbf{Homework/Worksheet 2 - Due: Wednesday, September 13}
    \end{center}
    % \begin{flushright}
    %     Fall 2023\quad \quad \quad \quad 
    % \end{flushright}
    
    


    \bigbreak \noindent \bigbreak \noindent 
    \textbf{1. Evaluate the Integrals}
    \bigbreak \noindent 
    \begin{mdframed}
        \textbf{1.a} $\int \frac{x^{3}}{\sqrt{1-x^{2}}} dx$
    \end{mdframed}
    \bigbreak \noindent 
    \begin{minipage}[t]{0.47\textwidth}
    \begin{align*}
        \text{Let $u=1-x^{2}$} \\
        du = -2x\ dx \\
        -\frac{1}{2}du = x\ dx \\
        x^{2} = -(u-1)
    .\end{align*}
    %\caption{}
    %\label{fig:}
    \end{minipage}
    \begin{minipage}[t]{0.37\textwidth}
    \begin{align*}
        &\int_{}^{}\ \frac{x^{3}}{\sqrt{1-x^{2}}}\ dx \\
        &=\int_{}^{}\ \frac{x(x^{2})}{\sqrt{1-x^{2}}}\ dx \\
        &=-\frac{1}{2}\int_{}^{}\ \frac{-(u-1)}{u^{\frac{1}{2}}}\ du \\
        &=\frac{1}{2}\int_{}^{}\ \frac{u-1}{u^{\frac{1}{2}}}\ du \\
        &=\frac{1}{2}\int_{}^{}\ (u-1)u^{-\frac{1}{2}}\ du \\
        &=\frac{1}{2}\int_{}^{}\ u^{\frac{1}{2}} - u^{-\frac{1}{2}}\ du \\
        &=\frac{1}{2}\bigg[\frac{2}{3}u^{\frac{3}{2}}-2^{\frac{1}{2}}\bigg] + C\\
        &=\frac{1}{3}u^{\frac{3}{2}} + u^{\frac{1}{2}} + C \\
        &= \frac{1}{3}(1-x^{2})^{\frac{3}{2}}-(1-x^{2})^{\frac{1}{2}}+ C \\
        &=\frac{(1-x^{2})^{\frac{3}{2}}}{3}-(1-x^{2})^{\frac{1}{2}} + C \\
        &=\frac{(1-x^{2})^{\frac{3}{2}}}{3} - \frac{3(1-x^{2})^{\frac{1}{2}}}{3} +C\\
        &= \frac{(1-x^{2})^{\frac{3}{2}}-3(1-x^{2})^{\frac{1}{2}}}{3} +C\\
        &= \frac{(1-x^{2})^{\frac{1}{2}}\big[(1-x^{2})-3\big]}{3} +C\\
        &= \frac{(1-x^{2})^{\frac{1}{2}}(-2-x^{2})}{3}+ C \\
        &= -\frac{1}{3}\sqrt{1-x^{2}}(2+x^{2}) + C
    .\end{align*}
    \end{minipage}


    \pagebreak \bigbreak \noindent 
    \begin{mdframed}
        \textbf{1.b} $\int_{}^{}\ \cos{x}(1-\cos{x})^{99}\sin{x}\ dx $
    \end{mdframed}
    \bigbreak \noindent 
    \begin{minipage}[t]{0.47\textwidth}
    \begin{align*}
        \text{Let $u=1-\cos{x}$} \\
        du = \sin{x}\ dx \\
        \cos{x} = -(u-1)
    .\end{align*}
    \end{minipage}
    \begin{minipage}[t]{0.52\textwidth}
        \begin{align*}
            &=\int_{}^{}\ \cos{x}(1-\cos{x})^{99}\sin{x}\ dx \\
            &=\int_{}^{}\ -(u-1)u^{99}\ du \\
            &=-\int_{}^{}\ (u-1)u^{99}\ du \\
            &=-\int_{}^{}\ u^{100}-u^{99}\ du \\
            &=-\bigg[\frac{1}{101}u^{101}-\frac{1}{100}u^{100}\bigg] + C \\
            &= -\frac{1}{101}(1-\cos{x})^{101}+\frac{1}{100}(1-\cos{x})^{100} + C
        .\end{align*}
    \end{minipage}



    \pagebreak \bigbreak \noindent 
    \begin{mdframed}
       \textbf{1.c} $\int_{}^{} \frac{x^{5}}{(1-x^{3})^{\frac{3}{2}}}\ dx $
    \end{mdframed}

    \bigbreak \noindent 
    \begin{minipage}[t]{0.47\textwidth}
    \begin{align*}
        \text{Let $u=1-x^{3}$} \\
        du = -3^{x2}\ dx\\
        -\frac{1}{3}du = x^{2}\ dx \\
        x^{3} = -(u-1)
    .\end{align*}
    %\caption{}
    %\label{fig:}
    \end{minipage}
    \begin{minipage}[t]{0.45\textwidth}
        \begin{align*}
           &\int \frac{x^{5}}{(1-x^{3})^{\frac{3}{2}}}\ dx \\
           &=\int \frac{x^{2}(x^{3})}{(1-x^{3})^{\frac{3}{2}}}\ dx  \\
           &=-\frac{1}{3}\int \frac{-(u-1)}{u^{3/2}}\ du \\
           &=\frac{1}{3}\int (u-1)u^{-\frac{3}{2}}\ du \\
           &=\frac{1}{3}\int u^{-\frac{1}{2}}-u^{-\frac{3}{2}}\ du \\
           &=\frac{1}{3}\bigg[2u^{\frac{1}{2}}+2u^{-\frac{1}{2}}\bigg] + C\\
           &=\frac{2}{3}u^{\frac{1}{2}}+\frac{2}{3}u^{-\frac{1}{2}} + C \\
           &= \frac{2}{3}(1-x^{3})^{\frac{1}{2}}+\frac{2}{3}(1-x^{3})^{-\frac{1}{2}} + C\\
           &=\frac{2}{3}(1-x^{3})^{\frac{1}{2}} + \frac{2}{3(1-x^{3})^{\frac{1}{2}}} + C \\
           &=\frac{2(1-x^{3})^{\frac{1}{2}}}{3} + \frac{2}{3(1-x^{3})^{\frac{1}{2}}} + C \\
           &=\frac{2(1-x^{3})^{\frac{1}{2}}(1-x^{3})^{\frac{1}{2}}+2}{3(1-x^{3})^{\frac{1}{2}}} + C  \\
           &=\frac{2(1-x^{3})+2}{3(1-x^{3})^{\frac{1}{2}}} + C \\
           &=\frac{4-2x^{3}}{3(1-x^{3})^{\frac{1}{2}}} +C\\
           &= -\frac{2(x^{3}-2)}{3(1-x^{3})^{\frac{1}{2}}} + C
        .\end{align*}
    %\caption{}
    %\label{fig:}
    \end{minipage}

    \pagebreak \bigbreak \noindent 

    \begin{mdframed}
        \textbf{1.d} $\int_{0}^{\frac{\pi}{4}}\ \sec^{2}{x}\tan{x}\ dx $
    \end{mdframed}
    \bigbreak \noindent 
    \begin{minipage}[t]{0.47\textwidth}
    \begin{align*}
        &\text{Let}\ u=\sec{x} \\
        &du = \sec{x}\tan{x} \\
        &u(a) = \sec{0} = 1 \\
        &u(b) = \sec{\frac{\pi}{4}} = \sqrt{2}
    .\end{align*}
    %\caption{}
    %\label{fig:}
    \end{minipage}
    \begin{minipage}[t]{0.45\textwidth}
    \begin{align*}
        &\int_{0}^{\frac{\pi}{4}}\ \sec^{2}{x}\tan{x}\ dx \\
        &=\int_{0}^{\frac{\pi}{4}}\ \sec{x}(\sec{x}\tan{x})\ dx \\
        &=\int_{1}^{\sqrt{2}}\ u\ du \\
        &=\frac{1}{2}u^{2}\bigg]^{\sqrt{2}}_{1} \\
        &= \frac{1}{2}\bigg((\sqrt{2})^{2}-(1)^{2}\bigg) \\
        &= \frac{1}{2}\bigg(2 - 1\bigg) \\
        &=\frac{1}{2}
    .\end{align*}
    %\caption{}
    %\label{fig:}
    \end{minipage}

    \bigbreak \noindent 
    \textbf{2. Evaluate the Integrals}

    \bigbreak \noindent 
    \begin{mdframed}
        \textbf{2.a} $\int e^{\sin{x}}\cos{x}\ dx $
    \end{mdframed}
    \bigbreak \noindent 
    \begin{minipage}[t]{0.47\textwidth}
    \begin{align*}
        &\text{Let}\ u=\sin{x} \\
        &du = \cos{x}
    .\end{align*}
    %\caption{}
    %\label{fig:}
    \end{minipage}
    \begin{minipage}[t]{0.36\textwidth}
    \begin{align*}
        &\int e^{\sin{x}}\cos{x}\ dx \\
        &=\int e^{u}\ du \\
        &=e^{\sin{x}} + C
    .\end{align*}
    %\caption{}
    %\label{fig:}
    \end{minipage}

    \bigbreak \noindent 
    \begin{mdframed}
        \textbf{2.b} $\int \frac{1}{x(\ln{x})}\ dx $
    \end{mdframed}
    \bigbreak \noindent 
    \begin{minipage}[t]{0.47\textwidth}
    \begin{align*}
        &\text{Let $u=\ln{x}$} \\
        &du = \frac{1}{x}\ dx
    .\end{align*}
    %\caption{}
    %\label{fig:}
    \end{minipage}
    \begin{minipage}[t]{0.37\textwidth}
    \begin{align*}
        &\int \frac{1}{x(\ln{x})}\ dx \\
        &=\int u^{-1}\ du \\
        &= \ln{\abs{u}} + C \\
        &= \ln{(\ln{\abs{x}})} + C
    .\end{align*}
    %\caption{}
    %\label{fig:}
    \end{minipage}

    \pagebreak 
    \begin{mdframed}
        \textbf{2.c} $\int xe^{-x^{2}}\ dx $
    \end{mdframed}
    \bigbreak \noindent 
    \begin{minipage}[t]{0.47\textwidth}
    \begin{align*}
        &\text{Let $u=-x^{2} $} \\
        &du =-2x \\
        &-\frac{1}{2}\ du = x\ dx
    .\end{align*}
    %\caption{}
    %\label{fig:}
    \end{minipage}
    \begin{minipage}[t]{0.36\textwidth}
    \begin{align*}
        & \int xe^{-x^{2}}\ dx \\
        &=-\frac{1}{2}\int e^{u}\ du \\
        &=-\frac{1}{2}e^{-x^{2}} + C
    .\end{align*}
    %\caption{}
    %\label{fig:}
    \end{minipage}

    \bigbreak \noindent 
    \begin{mdframed}
        \textbf{2.d} $\int \ln{(\cos{(x)})}\tan{x}\ dx $ 
    \end{mdframed}
    \begin{minipage}[t]{0.47\textwidth}
    \begin{align*}
        &\text{Let $u = \ln{(\cos{(x)})} $} \\
        &du = \frac{1}{\cos{x}}-\sin{x}\ dx \\
        &du = -\tan{x}\ dx \\
        &-du = \tan{x}\ dx
    .\end{align*}
    %\caption{}
    %\label{fig:}
    \end{minipage}
    \begin{minipage}[t]{0.44\textwidth}
    \begin{align*}
        &\int \ln{(\cos{(x)})}\tan{x}\ dx \\
        &=-\int u\ du \\
        &= -\frac{1}{2}u^{2} + C \\
        &=-\frac{1}{2}(\ln{(\cos{(x)})^{2}}) + C \\
        &=-\frac{1}{2}\ln^{2}{(\cos{(x)})} + C
    .\end{align*}
    %\caption{}
    %\label{fig:}
    \end{minipage}

    \bigbreak \noindent 
    \textbf{3. Evaluate the Integrals}
    \bigbreak \noindent 
    \begin{mdframed}
        \textbf{3.a} $\int_{-\frac{1}{2}}^{\frac{1}{2}}\ \frac{1}{\sqrt{1-x^{2}}}\ dx $
    \end{mdframed}
    \bigbreak \noindent 
    % \begin{remark}
    %     $\int \frac{1}{\sqrt{a^{2}-x^{2}}}\ dx = \sin^{-1}{\frac{x}{\abs{a}}} + C$ 
    % \end{remark}
    \bigbreak \noindent 
    \begin{align*}
        &\int_{-\frac{1}{2}}^{\frac{1}{2}}\ \frac{1}{\sqrt{1-x^{2}}}\ dx \\
        &=\sin^{-1}{x}\bigg]^{\frac{1}{2}}_{-\frac{1}{2}} \\
        &= \bigg(\frac{\pi}{6}-\bigg(-\frac{\pi}{6}\bigg)\bigg) \\
        &=\frac{2\pi}{6} \\
        &= \frac{\pi}{3}
    .\end{align*}

    \pagebreak 
    \begin{mdframed}
       \textbf{3.b} $\int_{}^{}\ \frac{1}{9+x^{2}}\ dx $ 
    \end{mdframed}
    \bigbreak \noindent 
    \begin{remark}
       $\int \frac{1}{x^{2}+a^{2}}\ dx  = \frac{1}{a}\tan^{-1}{\frac{x}{a}}+ C$
    \end{remark}
    \begin{align*}
        &\int \frac{1}{9+x^{2}}\ dx \\
        &= \frac{1}{3}\tan^{-1}{\frac{x}{3}} + C
    .\end{align*}

    \bigbreak \noindent 
    \begin{mdframed}
        \textbf{3.c} $\int \frac{\sin^{-1}{x}}{\sqrt{1-x^{2}}}\ dx $
    \end{mdframed}
    \bigbreak \noindent 
    \begin{minipage}[t]{0.47\textwidth}
    \begin{align*}
        &\text{Let $u=\sin^{-1}{x}$} \\
        &du = \frac{1}{\sqrt{1-x^{2}}}\ dx 
    .\end{align*}
    %\caption{}
    %\label{fig:}
    \end{minipage}
    \begin{minipage}[t]{0.35\textwidth}
    \begin{align*}
        &\int \frac{\sin^{-1}{x}}{\sqrt{1-x^{2}}}\ dx  \\
        &=\int u\ du \\
        &=\frac{1}{2}u^{2} + C \\
        &= \frac{1}{2}(\sin^{-1}{(x)})^{2} + C
    .\end{align*}
    %\caption{}
    %\label{fig:}
    \end{minipage}

    \bigbreak \noindent 
    \begin{mdframed}
        \textbf{3.d} $\int \frac{x\tan^{-1}{(x^{2})}}{1+ x^{4}}\ dx $
    \end{mdframed}
    \bigbreak \noindent 
    \begin{minipage}[t]{0.47\textwidth}
    \begin{align*}
        &\text{Let $u=\tan^{-1}{x^{2}}$} \\
        &du = \frac{1}{1+(x^{2})^{2}}\cdot 2x\ dx \\
        &du = \frac{2x}{1+x^{4}}\ dx \\
        &\frac{1}{2}du = \frac{x}{1+x^{4}}\ dx
    .\end{align*}
    %\caption{}
    %\label{fig:}
    \end{minipage}
    \begin{minipage}[t]{0.37\textwidth}
    \begin{align*}
        &\int \frac{x\tan^{-1}{(x^{2})}}{1+ x^{4}}\ dx \\
        &=\frac{1}{2}\int u\ du \\
        &=\frac{1}{2}\bigg[\frac{1}{2}u^{2}\bigg] + C \\
        &=\frac{1}{4}\bigg(\tan^{-1}{(x^{2})}\bigg)^{2} + C
    .\end{align*}
    %\caption{}
    %\label{fig:}
    \end{minipage}
    

    


    
\end{document}
