\documentclass{report}

\input{~/dev/latex/template/preamble.tex}
\input{~/dev/latex/template/macros.tex}

\title{\Huge{3.5 HW Solutions}}
\author{\huge{Nathan Warner}}
\date{\huge{Feb 28, 2023}}
\pagestyle{fancy}
\fancyhf{}
\rhead{MATHEMATICS HW SOLUTIONS}
\lhead{\leftmark}
\cfoot{\thepage}

\pgfpagesdeclarelayout{boxed}
{
  \edef\pgfpageoptionborder{0pt}
}
{
  \pgfpagesphysicalpageoptions
  {%
    logical pages=1,%
  }
  \pgfpageslogicalpageoptions{1}
  {
    border code=\pgfsetlinewidth{1.5pt}\pgfstroke,%
    border shrink=\pgfpageoptionborder,%
    resized width=.95\pgfphysicalwidth,%
    resized height=.95\pgfphysicalheight,%
    center=\pgfpoint{.5\pgfphysicalwidth}{.5\pgfphysicalheight}%
  }%
}

\pgfpagesuselayout{boxed}

\begin{document}
    \maketitle
    \begin{Large}
        \noindent \textbf{Question 1:}
    \end{Large}
    \bigbreak \noindent 
    \pf{Solution}{}
    \bigbreak \noindent 
    \textbf{\textit{\underline{Part 1:}}}
    \begin{align*}
        45x^{8}+7y^{6}\cdot \frac{dy}{dx}=4 \\
        = 7y^{6}\frac{dy}{dx} = -45x^{8} +4 \\
        = \frac{dy}{dx} = \frac{-45x^{8}+4}{7y^{6}}
    .\end{align*}
    \bigbreak \noindent 
    \textbf{\textit{\underline{Part 2: (solve for y)}}}
    \begin{align*}
        y^{7} = -5x^{9}+4x  \\
        y = (-5x^{9}+4x)^{\frac{1}{7}}
    .\end{align*}
    \begin{align*}
        y^{\prime} = \frac{1}{7}(-5x^{9}+4x)^{-\frac{6}{7}} \cdot (-45x^{8}+4) \\ 
        = \frac{-45x^{8}+4}{7(-5x^{9}+4x)^{\frac{6}{7}}}
    .\end{align*}
    \textbf{\textit{\underline{Part 3: Plug in what we got when we solved for y in part b into part a's y in the denominator:}}}
    \begin{align*}
        = \frac{dy}{dx} = \frac{-45x^{8}+4}{7[(-5x^{9}+4x)^{\frac{1}{7}}]^{6}}\\
        = \frac{dy}{dx} = \frac{-45x^{8}+4}{7(-5x^{9}+4x)^{\frac{6}{7}}}\\
    .\end{align*}


    \bigbreak \noindent \bigbreak \noindent 
    \begin{Large}
        \textbf{Question 2:}
    \end{Large}
    \bigbreak \noindent 
    \pf{Solution}{}
    \bigbreak \noindent 
    \textbf{\textit{\underline{Part 1:}}}
    \begin{align*}
      \frac{1}{2\sqrt{x}} + \frac{1}{2\sqrt{y}}\frac{dy}{dx} = 0  \\
      =\frac{1}{2\sqrt{y}}\frac{dy}{dx} = - \frac{1}{2\sqrt{x}} \\
      = \frac{dy}{dx}= -\frac{2\sqrt{y}}{2\sqrt{x}} \\
      = \frac{dy}{dx}= -\frac{\sqrt{y}}{\sqrt{x}} 
    .\end{align*}
    \bigbreak \noindent 
    \textbf{\textit{\underline{Part 2: Solve for y and differentiate}}}
    \begin{align*}
      y = (-\sqrt{x}+3)^{2}
    .\end{align*}
    \begin{align*}
      y^{\prime} = 2(-\sqrt{x}+3) \cdot (-\frac{1}{2}x^{-\frac{1}{2}}) \\ 
      = \frac{-2(-x^{\frac{1}{2}} + 3)}{2x^{\frac{1}{2}}} \\
      = \frac{-(-x^{\frac{1}{2}}+ 3)}{x^{\frac{1}{2}}} \\ 
      = \frac{x^{\frac{1}{2}}- 3}{x^{\frac{1}{2}}} \\ 
    .\end{align*}
    \bigbreak \noindent 
    \textbf{\textit{\underline{Part 3: Plug what we got when we solved for y in part b into the y from $y^{\prime}$ in part 1 }}}
    \begin{align*}
      y^{\prime} = \frac{-\sqrt{(-x^{\frac{1}{2}}+3)^{2}}}{x^{\frac{1}{2}}} \\
      y^{\prime} = \frac{-(-x^{\frac{1}{2}}+3)}{x^{\frac{1}{2}}} \\
      y^{\prime} = \frac{x^{\frac{1}{2}}-3}{x^{\frac{1}{2}}} \\
    .\end{align*}




    \bigbreak \noindent \bigbreak \noindent 
    \begin{Large}
        \textbf{Question 3:}
    \end{Large}
    \bigbreak \noindent 
    \pf{Solution}{}
    \bigbreak \noindent 
    \textbf{\textit{\underline{Part 1:}}}
    \begin{align*}
      y^{\prime} = 5x^{-2} + y^{-2} = 0 \\
      = -\frac{5}{x^{2}} + \frac{1}{y^{2}} = 0  \\
      = \frac{1}{y^{2}} = \frac{5}{x^{2}}  \\
      =  \frac{5y^{2}}{x^{2}}  \\
    .\end{align*}
    \textbf{\textit{\underline{Part 2: Solve for y:}}}
    \begin{align*}
      y= \\
      -\frac{1}{y} = -\frac{5}{x}  +4 \\
      -\frac{1}{y} = -\frac{5}{x} + 4 \\ 
      -\frac{1}{y} \cdot xy = -\frac{5}{x} \cdot xy +4 \cdot xy \\
        -\frac{xy}{y} = -\frac{5xy}{x} + 4xy \\
        -x = -5y+4xy \\
        -x = y(-5+4x) \\
        \frac{-x}{-5+4x} = y \\
        y = \frac{-x}{-5+4x}
   .\end{align*}
   \bigbreak \noindent 
   \textit{Now plug in y into the y in $y^{\prime}$ from part 1:}
   \begin{align*}
     y^{\prime} = \frac{5(-\frac{x}{4x-5})^{2}}{x^{2}} \\
     = \frac{5(-1)^{2}\frac{x^{2}}{(-5+4x)^{2}}}{x^{2}} \\
     = \frac{\frac{5x^{2}}{(-5+4x)^{2}}}{x^{2}} \\
     = \frac{5x^{2}}{(-5+4x)^{2}} \cdot \frac{1}{x^{2}} \\
     = \frac{5x^{2}}{(-5+4x)^{2}x^{2}} \\
     = \frac{5}{(-5+4x)^{2}}
   .\end{align*}


    \bigbreak \noindent \bigbreak \noindent 
    \begin{Large}
        \textbf{Question 4:}
    \end{Large}
    \bigbreak \noindent 
    \pf{Solution}{}
    \bigbreak \noindent 
    \begin{align*}
      2x-10x \frac{dy}{dx}-10y+2y \frac{dy}{dx} = 0 \\
      = \frac{dy}{dx}(-10x+2y) = -2x + 10y \\
      \frac{dy}{dx} = \frac{-2x+10y}{-10x+2y} \\
      \frac{dy}{dx} = \frac{2(-x+5y)}{2(-5x+y)} \\
      \frac{dy}{dx} = \frac{-x+5y}{-5x+y} \\
    .\end{align*}


    \bigbreak \noindent \bigbreak \noindent 
    \begin{Large}
        \textbf{Question 5:}
    \end{Large}
    \bigbreak \noindent 
    \pf{Solution}{}
    \bigbreak \noindent 
    \begin{align*}
      -y\sin{x}+\frac{dy}{dx}\cos{x} = 6x+10y \frac{dy}{dx} \\
      = \frac{dy}{dx}(cosx-10y) = 6x+y\sin{x} \\
      = \frac{dy}{dx} = \frac{6x+y\sin{x}}{\cos{x}-10y}
    .\end{align*}


    \bigbreak \noindent \bigbreak \noindent 
    \begin{Large}
        \textbf{Question 6:}
    \end{Large}
    \bigbreak \noindent 
    \pf{Solution}{}
    \bigbreak \noindent 
    \begin{align*}
      e^{\frac{x}{y}} \cdot \frac{y}{x} = 2 - \frac{dy}{dx} \\
      e^{\frac{x}{y}}(\frac{y \cdot 1 - x \cdot \frac{dy}{dx}}{y^{2}}) = 2 - \frac{dy}{dx} \\
      e^{\frac{x}{y}}(\frac{y - x \cdot \frac{dy}{dx}}{y^{2}}) = 2-\frac{dy}{dx}\\
      e^{\frac{x}{y}}(\frac{y}{y^{2}} - \frac{x}{y^{2}}\frac{dy}{dx}) = 2- \frac{dy}{dx}\\
      e^{\frac{x}{y}}(\frac{y}{y^{2}} - \frac{x}{y^{2}}\frac{dy}{dx}) = 2 - \frac{dy}{dx} \\
      e^{\frac{x}{y}}(\frac{1}{y} - \frac{x}{y^{2}}\frac{dy}{dx}) = 2 - \frac{dy}{dx} \\
      \frac{1}{y}e^{\frac{x}{y}}-\frac{x}{y^{2}}e^{\frac{x}{y}}\frac{dy}{dx} = 2-\frac{dy}{dx} \\
      \frac{dy}{dx} -\frac{x}{y^{2}}e^{\frac{x}{y}} \frac{dy}{dx} = 2 - \frac{1}{y}e^{\frac{x}{y}} \\
      \frac{dy}{dx}(1 -\frac{x}{y^{2}}e^{\frac{x}{y}}) = 2 - \frac{1}{y}e^{\frac{x}{y}} \\
      \frac{dy}{dx} = \frac{2- \frac{1}{y}e^{\frac{x}{y}}}{(1 -\frac{x}{y^{2}}e^{\frac{x}{y}})} \\
    .\end{align*}
    \textit{From here multiply by common denominator $y^{2}$ to clear out the fractions:}
    \begin{align*}
      \frac{2y^{2} - ye^{\frac{x}{y}}}{y^{2}-xe^{\frac{x}{y}}} \\
    \frac{dy}{dx} = \frac{y(2y-e^{\frac{x}{y}})}{y^{2}-xe^{\frac{x}{y}}}
    .\end{align*}


    \bigbreak \noindent \bigbreak \noindent 
    \begin{Large}
        \textbf{Question 7:}
    \end{Large}
    \bigbreak \noindent 
    \pf{Solution}{}
    \bigbreak \noindent 


    \bigbreak \noindent \bigbreak \noindent 
    \begin{Large}
        \textbf{Question 8:}
    \end{Large}
    \bigbreak \noindent 
    \pf{Solution}{}
    \bigbreak \noindent 


    \bigbreak \noindent \bigbreak \noindent 
    \begin{Large}
        \textbf{Question 9:}
    \end{Large}
    \bigbreak \noindent 
    \pf{Solution}{}
    \bigbreak \noindent 


    \bigbreak \noindent \bigbreak \noindent 
    \begin{Large}
        \textbf{Question 10:}
    \end{Large}
    \bigbreak \noindent 
    \pf{Solution}{}
    \bigbreak \noindent 


    \bigbreak \noindent \bigbreak \noindent 
    \begin{Large}
        \textbf{Question 11:}
    \end{Large}
    \bigbreak \noindent 
    \pf{Solution}{}
    \bigbreak \noindent 


\end{document}
