\documentclass{report}

\input{~/dev/latex/template/preamble.tex}
\input{~/dev/latex/template/macros.tex}

\title{\Huge{3.4 Hw Solutions}}
\author{\huge{Nathan Warner}}
\date{\huge{Feb 22, 2023}}

\pgfpagesdeclarelayout{boxed}
{
  \edef\pgfpageoptionborder{0pt}
}
{
  \pgfpagesphysicalpageoptions
  {%
    logical pages=1,%
  }
  \pgfpageslogicalpageoptions{1}
  {
    border code=\pgfsetlinewidth{1.5pt}\pgfstroke,%
    border shrink=\pgfpageoptionborder,%
    resized width=.95\pgfphysicalwidth,%
    resized height=.95\pgfphysicalheight,%
    center=\pgfpoint{.5\pgfphysicalwidth}{.5\pgfphysicalheight}%
  }%
}

\pgfpagesuselayout{boxed}

\begin{document}
    \maketitle
    \begin{Large}
        \noindent \textbf{Question 1:}
    \end{Large}
    \bigbreak \noindent 
    \pf{Solution}{}
    \bigbreak \noindent 
    \begin{align*}
        y^{\prime} = 9(6-x^3)^{8} \cdot (-3x^{2}) \\
        = -27(6-x^{3})^{8}
    .\end{align*}

    \bigbreak \noindent \bigbreak \noindent 
    \begin{Large}
        \textbf{Question 2:}
    \end{Large}
    \bigbreak \noindent 
    \pf{Solution}{}
    \bigbreak \noindent 
    \begin{align*}
        y^{\prime} = \sec^{2}{x^{5}} \cdot 5x^{4} \\ 
        = 5x^{4}\sec^{2}{x^{5}}
    .\end{align*}

    \bigbreak \noindent \bigbreak \noindent 
    \begin{Large}
        \textbf{Question 3:}
    \end{Large}
    \bigbreak \noindent 
    \pf{Solution}{}
    \bigbreak \noindent 
    \begin{align*}
        e^{5x^{\frac{1}{2}}} \cdot \frac{5}{2}x^{-\frac{1}{2}} \\
        \frac{5}{2}x^{-\frac{1}{2}}e^{5x^{\frac{1}{2}}} \\
        = \frac{5e^{5x^{\frac{1}{2}}}}{2x^{\frac{1}{2}}}
    .\end{align*}

    \bigbreak \noindent \bigbreak \noindent 
    \begin{Large}
        \textbf{Question 4:}
    \end{Large}
    \bigbreak \noindent 
    \pf{Solution}{}
    \bigbreak \noindent 
    \textbf{\textit{\underline{Part 1:}}}
    \begin{align*}
        g^{\prime}(x) = 6x^2-16x 
    .\end{align*}
    \bigbreak \noindent 
    \textbf{\textit{\underline{Part 2:}}}
    \begin{align*}
        6(2x^{3}-8x^{2}+9)^5 \cdot (6x^{2}-16x) \\
        = 6(2x^{3}-8x^{2}+9)^5 \cdot 2(3x^{2}-8x) \\
        = 12(2x^{3}-8x^{2}+9)^5 \cdot (3x^{2}-8x) \\
    .\end{align*}

    \bigbreak \noindent \bigbreak \noindent 
    \begin{Large}
        \textbf{Question 5:}
    \end{Large}
    \bigbreak \noindent 
    \pf{Solution}{}
    \bigbreak \noindent 
    \begin{align*}
        f(x) = 1 \\
        f^{\prime}(x) = 0 
    .\end{align*}
    \begin{align*}
        g(x) = (2x^2-5)^{\frac{1}{3}} \\
        g^{\prime}(x) = \frac{1}{3}(2x^{2}-5)^{-\frac{2}{3}} \cdot 4x
    .\end{align*}
    \begin{align*}
        F^{\prime}(x) = \frac{(2x^{2}-5)^{\frac{1}{3}}(0) - (1)[\frac{1}{3}(2x^{2}-5)^{-\frac{2}{3}}(4x)]}{(2x^{2}-5)^{\frac{2}{3}}} \\
        = \frac{(2x^{2}-5)^{\frac{1}{3}}(0) - (1)[\frac{1}{3}(2x^{2}-5)^{-\frac{2}{3}}(4x)]}{(2x^{2}-5)^{\frac{2}{3}}} \\
        = \frac{- \frac{4}{3}x(2x^{2}-5)^{-\frac{2}{3}}}{(2x^{2}-5)^{\frac{2}{3}}} \\ 
        = \frac{-\frac{4}{3}x}{(2x^{2}-5)^{\frac{4}{3}}} \\
        = -\frac{4x}{3(2x^{2}-5)^{\frac{4}{3}}} \\
    .\end{align*}

    \bigbreak \noindent \bigbreak \noindent 
    \begin{Large}
        \textbf{Question 6:}
    \end{Large}
    \bigbreak \noindent 
    \pf{Solution}{}
    \bigbreak \noindent 
    \begin{align*}
        F(t) = (9t+1)^{-5}
    .\end{align*}
    \begin{align*}
        F^{\prime}(t) = -5(9t+1)^{-6} \cdot 9 \\
        = -45(9t+1)^{-6} \\
        = -\frac{45}{(9t+1)^{6}}
    .\end{align*}

    \bigbreak \noindent \bigbreak \noindent 
    \begin{Large}
        \textbf{Question 7:}
    \end{Large}
    \bigbreak \noindent 
    \pf{Solution}{}
    \bigbreak \noindent 
    \textbf{\textit{\underline{Move the constant outside:}}}
    \begin{align*}
        7(\cos^{3}{\theta})
    .\end{align*}
    \begin{align*}
        \frac{d}{d\theta} = 7(\cos{\theta })^{3} \\
        = 7 \cdot 3(\cos{\theta })^{2} \cdot -\sin{\theta} \\
        -21\cos^{2}{\theta} \sin{\theta }
    .\end{align*}

    \bigbreak \noindent \bigbreak \noindent 
    \begin{Large}
        \textbf{Question 8:}
    \end{Large}
    \bigbreak \noindent 
    \pf{Solution}{}
    \bigbreak \noindent 
    \begin{align*}
        e^{x^{4}-5x}(4x^{3}-5)
    .\end{align*}

    \bigbreak \noindent \bigbreak \noindent 
    \begin{Large}
        \textbf{Question 9:}
    \end{Large}
    \bigbreak \noindent 
    \pf{Solution}{}
    \bigbreak \noindent 
    \begin{align*}
        f(x) = (4x+5)^{3} \\
        f^{\prime}(x) = 3(4x+5)^{2}(4)
    .\end{align*}
    \begin{align*}
        g(x) = (x^{2}-8x+5)^{4} \\
        g^{\prime}(x) = 4(x^{2}-8x+5)^{3}(2x-8)
    .\end{align*}
    \begin{align*}
        F^{\prime}(x) = (4x+5)^{3}[4(x^{2}-8x+5)^{3}(2x-8)]+(x^{2}-8x+5)^{4}[3(4x+5)^{2}\cdot 4] \\
        = (4x+5)^{2}(x^{2}+8x+5)^{3}[4(4x+5)(2x-8)+12(x^{2}-8x+5)]\\
        = (4x+5)^{2}(x^{2}+8x+5)^{3}[4(8x^2-22x-40)+12x^{2}-96x+60]\\
        = (4x+5)^{2}(x^{2}+8x+5)^{3}[32x^2-88x-160+12x^{2}-96x+60]\\
        = (4x+5)^{2}(x^{2}+8x+5)^{3}[44x^{2}-184x-100]\\
        = (4x+5)^{2}(x^{2}+8x+5)^{3}[4(11x^{2}-46x-25)]\\
        = 4(4x+5)^{2}(x^{2}+8x+5)^{3}(11x^{2}-46x-25)\\
    .\end{align*}


    \bigbreak \noindent \bigbreak \noindent 
    \begin{Large}
        \textbf{Question 10:}
    \end{Large}
    \bigbreak \noindent 
    \pf{Solution}{}
    \bigbreak \noindent 
    \begin{align*}
      f(x) = (u^{3}-3)^{9} \\
      f^{\prime}(x) = 9(u^{3}-3)^{8}(3u^{2})
    .\end{align*}
    \begin{align*}
      g(x) = (u^{3}+3)^{9} \\
      g^{\prime}(x) = 9(u^{3}+3)^{8}(3u^{2})
    .\end{align*}
    \begin{align*}
      G^{\prime}(x) = \frac{(u^{3}+3)^{9}[9(u^{3}-3)^{8}(3u^{2})]-(u^{3}-3)^{9}[9(u^{3}+3)^{8}(3u^{2})]}{(u^{3}+3)^{18}}\\
      = \frac{(u^{3}-3)^{8}(u^{3}+3)^{8}(3u^{2})[9(u^{3}+3)^8]-[9(u^{3}-3)]}{(u^{3}+3)^{18}} \\
      = \frac{(u^{3}-3)^{8}(3u^{2})[9(u^{3}+3)-[9(u^{3}-3)]]}{(u^{3}+3)^{10}} \\
      = \frac{(u^{3}-3)^{8}(3u^{2})[9(u^{3}+3)-(9u^{3}-27)]}{(u^{3}+3)^{10}} \\
      = \frac{(u^{3}-3)^{8}(3u^{2})[9u^{3}+27-(9u^{3}-27)]}{(u^{3}+3)^{10}} \\
      = \frac{(u^{3}-3)^{8}(3u^{2})(9u^{3}+27-9u^{3}+27)}{(u^{3}+3)^{10}} \\
      = \frac{(u^{3}-3)^{8}(3u^{2})(27+27)}{(u^{3}+3)^{10}} \\
      = \frac{(u^{3}-3)^{8}(3u^{2})(54)}{(u^{3}+3)^{10}} \\
      = \frac{(u^{3}-3)^{8}162u^{2}}{(u^{3}+3)^{10}} \\
      = \frac{162u^{2}(u^{3}-3)^{8}}{(u^{3}+3)^{10}} \\
    .\end{align*}


    \bigbreak \noindent \bigbreak \noindent 
    \begin{Large}
        \textbf{Question 11:}
    \end{Large}
    \bigbreak \noindent 
    \pf{Solution}{}
    \bigbreak \noindent 
    \begin{align*}
      \ln{7}\cdot \ln{8}\cdot \ln{9} \cdot 7^{8^{9^{x}}} \cdot 8^{9^{x}} \cdot 9^{x} 
    .\end{align*}

    \bigbreak \noindent \bigbreak \noindent 
    \begin{Large}
        \textbf{Question 12:}
    \end{Large}
    \bigbreak \noindent 
    \pf{Solution}{}
    \bigbreak \noindent 
    \textbf{\textit{\underline{Part 1:}}}
    \begin{align*}
      -\sin{(\sin{9\theta})} \cdot 9\cos{9\theta } \\
      = -9\cos{9\theta }\sin{(\sin{9\theta })}
    .\end{align*}
    \bigbreak \noindent 
    \textbf{\textit{\underline{Part 2:}}}
    \begin{align*}
      f(x) = \cos{9\theta } \\
      f^{\prime}(x) = -9\sin{9\theta }
    .\end{align*}
    \begin{align*}
      g(x) = \sin{\sin{9\theta}} \\
      g^{\prime}(x) = \cos{(\sin{9\theta })} \cdot 9\cos{9\theta }
    .\end{align*}
    \begin{align*}
      -9(\cos{9\theta } \cdot \cos{(\sin{9\theta })\cdot 9\cos{9\theta }} + \sin{(\sin{9\theta })} \cdot  -9\sin{9\theta }) \\
      -9(9\cos^{2}{9\theta } \cdot \cos{(\sin{9\theta }})+ \sin{(\sin{9\theta })} \cdot  -9\sin{9\theta }) \\
      -9(9\cos^{2}{9\theta } \cdot \cos{(\sin{9\theta }})-9\sin{(\sin{9\theta })} \cdot \sin{9\theta }) \\
      -81\cos^{2}{9\theta } \cdot \cos{(\sin{9\theta }})+81\sin{(\sin{9\theta })} \cdot \sin{9\theta } \\
    .\end{align*}


    \bigbreak \noindent \bigbreak \noindent 
    \begin{Large}
        \textbf{Question 13:}
    \end{Large}
    \bigbreak \noindent 
    \pf{Solution}{}
    \bigbreak \noindent 
    \textbf{\textit{\underline{By the shortcut:}}}
    \begin{align*}
      \frac{d}{dx}\sqrt{5+x^{3}} \\
      = \frac{3x^{2}}{2(5+x^{3})^{\frac{1}{2}}}
    .\end{align*}
    \textbf{\textit{\underline{Part 2:}}}
    \begin{align*}
      \frac{3(-1)^{2}}{2(5+(-1)^{3})^{\frac{1}{2}}} \\
      = \frac{3}{4}
    .\end{align*}
    \begin{align*}
      y - 2 = \frac{3}{4}(x-(-1)) \\
      y - 2 = \frac{3}{4}(x+1) \\
      y - 2 = \frac{3}{4}x+\frac{3}{4} \\
      y = \frac{3}{4}x+\frac{11}{4} \\
    .\end{align*}

    \bigbreak \noindent \bigbreak \noindent 
    \begin{Large}
        \textbf{Question 14:}
    \end{Large}
    \bigbreak \noindent 
    \pf{Solution}{}
    \bigbreak \noindent 
    \textbf{\textit{\underline{By the shortcut:}}}
    \begin{align*}
      y^{\prime} = \frac{1}{(-6+2x)^{\frac{1}{2}}}
    .\end{align*}
    \textbf{\textit{\underline{Part 2:}}}
    \begin{align*}
      If\ 8x+4y = 1 \\
    .\end{align*}
    \begin{center}
      And
    \end{center}
    \begin{align*}
      m = \frac{-a}{b} 
    .\end{align*}
    \begin{center}
      Then:
    \end{center}
    \begin{align*}
      m = -\frac{8}{4} \\ 
      m = -2
    .\end{align*}
    \begin{align*}
      \sqrt{-6+2x} = 2 \\ 
      -6+2x=4 \\ 
      2x=10 \\
      x =5 \\
      so\
      (5,2)
    .\end{align*}


    \bigbreak \noindent \bigbreak \noindent 
    \begin{Large}
        \textbf{Question 15:}
    \end{Large}
    \bigbreak \noindent 
    \pf{Solution}{}
    \bigbreak \noindent 
    \begin{align*}
      f^{\prime}(g(x)) \cdot g^{\prime}(x) \\
      = 9 \cdot 2 \\
      18
    .\end{align*}

    \bigbreak \noindent \bigbreak \noindent 
    \begin{Large}
        \textbf{Question 16:}
    \end{Large}
    \bigbreak \noindent 
    \pf{Solution}{}
    \bigbreak \noindent 
    \begin{align*}
      F^{\prime}(2) = f^{\prime}(2) \cdot f^{\prime}(f(2)) \\
      = 5 \cdot f^{\prime}(1) \\ 
      = 5 \cdot 4 \\
      = 20
    .\end{align*}
    \begin{align*}
      G^{\prime}(3) = g^{\prime}(3) \cdot g^{\prime}(g(3)) \\
      = 9 \cdot g^{\prime}(1) \\ 
      = 9 \cdot 6 \\
      = 54
    .\end{align*}

    \bigbreak \noindent \bigbreak \noindent 
    \begin{Large}
        \textbf{Question 17:}
    \end{Large}
    \bigbreak \noindent 
    \pf{Solution}{}
    \bigbreak \noindent 
    
\end{document}
