\documentclass{report}

\input{~/dev/latex/template/preamble.tex}
\input{~/dev/latex/template/macros.tex}

\title{\Huge{}}
\author{\huge{Nathan Warner}}
\date{\huge{}}
\fancyhf{}
\rhead{}
\fancyhead[R]{\itshape Warner} % Left header: Section name
\fancyhead[L]{\itshape\leftmark}  % Right header: Page number
\cfoot{\thepage}
\renewcommand{\headrulewidth}{0pt} % Optional: Removes the header line
%\pagestyle{fancy}
%\fancyhf{}
%\lhead{Warner \thepage}
%\rhead{}
% \lhead{\leftmark}
%\cfoot{\thepage}
%\setborder
% \usepackage[default]{sourcecodepro}
% \usepackage[T1]{fontenc}

% Change the title
\hypersetup{
    pdftitle={Relative error 3 proof}
}

\begin{document}
    % \maketitle
    %     \begin{titlepage}
    %    \begin{center}
    %        \vspace*{1cm}
    % 
    %        \textbf{}
    % 
    %        \vspace{0.5cm}
    %         
    %             
    %        \vspace{1.5cm}
    % 
    %        \textbf{Nathan Warner}
    % 
    %        \vfill
    %             
    %             
    %        \vspace{0.8cm}
    %      
    %        \includegraphics[width=0.4\textwidth]{~/niu/seal.png}
    %             
    %        Computer Science \\
    %        Northern Illinois University\\
    %        United States\\
    %        
    %             
    %    \end{center}
    % \end{titlepage}
    % \tableofcontents
    % \pagebreak 

    \bigbreak \noindent \bigbreak \noindent \bigbreak \noindent 
    \noindent \textbf{Theorem} \textit{\textit{(Relative error bound III).}}  Let $A$ be nonsingular, $b\ne 0$, and $Ax=b$. If $(A + \delta A)(x + \delta x) = b + \delta  b$, and 
        \begin{align*}
            \frac{\norm{\delta  A}}{\norm{A}} < \frac{1}{\kappa(A)},
        \end{align*}
        then
        \begin{align*}
            \frac{\norm{\delta x}}{\norm{x}} \leq \frac{\kappa(A)\left(\frac{\norm{\delta A}}{\norm{A}} + \frac{\norm{\delta b}}{\norm{b}}\right)}{1-\kappa(A)\frac{\norm{\delta A}}{\norm{A}}}
        .\end{align*}
        \bigbreak \noindent 
        \begin{remark}[a] Consider the quantity $q = \frac{a}{b}$, $b\ne 0$. If $c \leq b$, then 
            \begin{align*}
                q = \frac{a}{b} \leq \frac{a}{c}
            .\end{align*}
            
        \end{remark} 
        
        \bigbreak \noindent 
        \textbf{\textit{Proof.}} Suppose for a moment that $A$ nonsingular, $b\ne 0$, $Ax= b$, and $(A + \delta A)(x + \delta x) = b + \delta b$. Then, it's easy to see that
        \begin{align*}
            (A+\delta A)(x + \delta x) &= b + \delta b \\
            \implies Ax + A\delta x + \delta Ax + \delta A \delta x &= b + \delta b\\
            \implies A\delta x + \delta Ax + \delta A \delta x &= \delta b\\
            \implies A\delta x &= \delta b - (\delta Ax + \delta A \delta x) \\
            \implies A\delta x &= \delta b - \delta A\left(x + \delta x\right) \\
            \implies \delta x &= A^{-1} \delta b - A^{-1}\delta A\left(x+\delta x\right) \\
            \implies \norm{\delta x} &= \norm{A^{-1}\delta b -A^{-1}\delta A\left(x + \delta x\right)} \\
                                     &\leq\norm{A^{-1}\delta b} + \norm{-A^{-1} \delta A\left(x + \delta x\right)} \\
                                     &=\norm{A^{-1}\delta b} + \norm{A^{-1} \delta A\left(x + \delta x\right)}  \\
                                     &\leq \norm{A^{-1}}\norm{\delta b} + \norm{A^{-1}}\norm{\delta A}\left(\norm{x + \delta x}\right) \\
                                     &\leq \norm{A^{-1}}\norm{\delta b} + \norm{A^{-1}}\norm{\delta A}\left(\norm{x} + \norm{\delta x}\right) \\
                                     &=\norm{A^{-1}}\norm{\delta b} + \norm{A^{-1}}\norm{\delta A}\norm{x} + \norm{A^{-1}}\norm{\delta A}\norm{\delta x} \\
            \implies \norm{\delta x} - \norm{A^{-1}}\norm{\delta A}\norm{\delta x} &\leq \norm{A^{-1}}\norm{\delta b} + \norm{A^{-1}}\norm{\delta A}\norm{x} \\
            \implies \norm{\delta x}\left(1-\norm{A^{-1}}\norm{\delta A}\right) &\leq \norm{A^{-1}}\norm{\delta b} + \norm{A^{-1}}\norm{\delta A}\norm{x} \\
            \implies \frac{\norm{A}}{\norm{A}}\norm{\delta x} \left(1-\norm{A^{-1}}\norm{\delta A}\right) &\leq \frac{\norm{A}}{\norm{A}}\left(\norm{A^{-1}}\norm{\delta b} + \norm{A^{-1}}\norm{\delta A}\norm{x}\right) \\
            \implies \norm{\delta x}\left(1-\norm{A}\norm{A^{-1}}\frac{\norm{\delta A}}{\norm{A}}\right) &\leq \norm{A}\norm{A^{-1}}\frac{\norm{\delta b}}{\norm{A}} + \norm{A}\norm{A^{-1}}\frac{\norm{\delta A}}{\norm{A}}\norm{x} \\
            \implies \norm{\delta x}\left(1-\kappa(A)\frac{\norm{\delta A}}{\norm{A}}\right) &\leq \kappa(A)\frac{\norm{\delta b}}{\norm{A}} + \kappa(A)\frac{\norm{\delta A}}{\norm{A}}\norm{x} \\ 
            \implies \frac{\norm{\delta x}}{\norm{x}}\left(1-\kappa(A)\frac{\norm{\delta A}}{\norm{A}}\right) &\leq \kappa(A)\frac{\norm{\delta b}}{\norm{A}\norm{x}} + \kappa(A)\frac{\norm{\delta A}}{\norm{A}}
        .\end{align*} 
        From here, we use 
        \begin{align*}
            Ax &= b \\
            \implies \norm{Ax} &= \norm{b} \\
            \implies \norm{Ax} &\leq \norm{A}\norm{x} \\
            \implies \norm{b} &\leq \norm{A}\norm{x}
        \end{align*}
        and remark \textit{(a)} to see that
        \begin{align*}
            \kappa(A) \frac{\norm{\delta b}}{\norm{A}\norm{x}} + \kappa(A) \frac{\norm{\delta A}}{\norm{A}} & \leq \kappa(A) \frac{\norm{\delta b}}{\norm{b}} + \kappa(A) \frac{\norm{\delta A}}{\norm{A}} 
        .\end{align*}
        Thus, it follows that
        \begin{align*}
            \frac{\norm{\delta x}}{\norm{x}}\left(1-\kappa(A)\frac{\norm{\delta A}}{\norm{A}}\right) &\leq \kappa(A)\frac{\norm{\delta b}}{\norm{A}\norm{x}} + \kappa(A)\frac{\norm{\delta A}}{\norm{A}} \\
                                                                                                              &\leq \kappa(A) \frac{\norm{\delta b}}{\norm{b}} + \kappa(A) \frac{\norm{\delta A}}{\norm{A}}  \\
                                                                                                              &= \kappa(A)\left(\frac{\norm{\delta b}}{\norm{b}}  + \frac{\norm{\delta A}}{\norm{A}}\right) \\
            \therefore \frac{\norm{\delta x}}{\norm{x}} &\leq \frac{\kappa(A)\left(\frac{\norm{\delta A}}{\norm{A}} + \frac{\norm{\delta b}}{\norm{b}}\right)}{1-\kappa(A)\frac{\norm{\delta A}}{\norm{A}}}
        .\end{align*}
        As desired. $\endpf$





\end{document}
