\documentclass{report}

\input{~/dev/latex/template/preamble.tex}
\input{~/dev/latex/template/macros.tex}

\title{\Huge{3.1 Hw Solutions}}
\author{\huge{Nathan Warner}}
\date{\huge{Feb 15, 2023}}

\pgfpagesdeclarelayout{boxed}
{
  \edef\pgfpageoptionborder{0pt}
}
{
  \pgfpagesphysicalpageoptions
  {%
    logical pages=1,%
  }
  \pgfpageslogicalpageoptions{1}
  {
    border code=\pgfsetlinewidth{1.5pt}\pgfstroke,%
    border shrink=\pgfpageoptionborder,%
    resized width=.95\pgfphysicalwidth,%
    resized height=.95\pgfphysicalheight,%
    center=\pgfpoint{.5\pgfphysicalwidth}{.5\pgfphysicalheight}%
  }%
}

\pgfpagesuselayout{boxed}

\begin{document}
    \maketitle
    \begin{Large}
        \noindent \textbf{Question 1:}
    \end{Large}
    \bigbreak \noindent 
    \pf{Solution}{}
    \bigbreak \noindent
    \begin{align*}
        g ^{\prime}(x) = 9 \cdot 1 - 0 \\ 
        = 9
    .\end{align*}

    \bigbreak \noindent \bigbreak \noindent 
    \begin{Large}
        \noindent \textbf{Question 2:}
    \end{Large}
    \bigbreak \noindent 
    \pf{Solution}{}
    \bigbreak \noindent 
    \begin{align*}
        g ^{\prime}(t) = 7(1) + 10t \\
        = 7 +10t
    .\end{align*}

    \bigbreak \noindent \bigbreak \noindent 
    \begin{Large}
        \noindent \textbf{Question 3:}
    \end{Large}
    \bigbreak \noindent 
    \pf{Solution}{}
    \bigbreak \noindent 
    \begin{align*}
        \frac{5}{8}(2)x^{2-1}-8(1)-0 \\
        = \frac{5}{4}x -8
    .\end{align*}

    \bigbreak \noindent \bigbreak \noindent 
    \begin{Large}
        \noindent \textbf{Question 4:}
    \end{Large}
    \bigbreak \noindent 
    \pf{Solution}{}
    \bigbreak \noindent 
    \begin{center}
        Since:
    \end{center}
    \begin{align*}
        \frac{d}{dx} e^x = e^x
    .\end{align*}
    \begin{align*}
        f ^{\prime}(t) = -5e^t
    .\end{align*}

    \bigbreak \noindent \bigbreak \noindent 
    \begin{Large}
        \noindent \textbf{Question 5:}
    \end{Large}
    \bigbreak \noindent 
    \pf{Solution}{}
    \bigbreak \noindent 
    \begin{align*}
        -4z^{-4-1} - \frac{1}{2}z^{^{ \frac{1}{2} - 1}} \\ 
        = -4z^{-5}- \frac{1}{2}z^{- ^{\frac{1}{2}}} \\ 
        = - \frac{4}{z^5} - \frac{1}{2z^{ \frac{1}{2}}}
    .\end{align*} 

    \bigbreak \noindent \bigbreak \noindent 
    \begin{Large}
        \noindent \textbf{Question 6:}
    \end{Large}
    \bigbreak \noindent 
    \pf{Solution}{}
    \bigbreak \noindent 
    \begin{align*}
        x^3(x+8) \\
        = x^4+8x^3 \\ 
        = 4x^3 +24x^2
    .\end{align*}

    \bigbreak \noindent \bigbreak \noindent 
    \begin{Large}
        \noindent \textbf{Question 7:}
    \end{Large}
    \bigbreak \noindent 
    \pf{Solution}{}
    \bigbreak \noindent 
    \begin{align*}
        8e^x + 5x^{ ^{-\frac{1}{3}}} \\
        = 8e^x+5(- \frac{1}{3})x^{ ^{-\frac{1}{3} - 1}} \\ 
        = 8e^x - \frac{5}{3}x^{ ^{-\frac{4}{3}}} \\
        = 8e^x - \frac{5}{3x^{ \frac{4}{3}}}
    .\end{align*}

    \bigbreak \noindent \bigbreak \noindent 
    \begin{Large}
        \noindent \textbf{Question 8:}
    \end{Large}
    \bigbreak \noindent 
    \pf{Solution}{}
    \bigbreak \noindent 
    \begin{align*}
        (8+q^{-1})(8+q^{-1}) \\ 
        =(8+ \frac{1}{q})(8+ \frac{1}{q}) \\
        =8 \cdot 8+2( \frac{8}{q}) + ( \frac{1}{q})^2 \\ 
        = 64+ \frac{16}{q} + \frac{1}{q^2} \\ 
        = 64 +16q^{-1} + q^{-2} \\ 
        = 0 -16q^{-2} -2q^{-3} \\ 
        = - \frac{16}{q^2} - \frac{2}{q^3}
    .\end{align*}

    \bigbreak \noindent \bigbreak \noindent 
    \begin{Large}
        \noindent \textbf{Question 9:}
    \end{Large}
    \bigbreak \noindent 
    \pf{Solution}{}
    \bigbreak \noindent 
    \begin{center}
      $e^{x+4}$ Gets left alone
    \end{center}
    \bigbreak \noindent 
    \textit{So:}
    \begin{align*}
      y ^{\prime} = e^{x+4} + 0 \\
      = e^{x+4}
    .\end{align*}
    \bigbreak \noindent \bigbreak \noindent 
    \begin{Large}
        \noindent \textbf{Question 10:}
    \end{Large}
    \bigbreak \noindent 
    \pf{Solution}{}
    \bigbreak \noindent 
    \bigbreak \noindent 
    \textit{$f ^{\prime}(x)$:}
    \begin{align*}
      f ^{\prime}(x) = 14x-3x^2
    .\end{align*}
    \bigbreak \noindent 
    \textit{$m_{tan}$:}
    \begin{align*}
      m_{tan} = 14(1)-3(1)^2 \\ 
      = 11
    .\end{align*}
    \bigbreak \noindent 
    \textit{Equation:}
    \begin{align*}
      y - 6 = 11(x-1) \\ 
      y -6 = 11x-11 \\ 
      y = 11x -5
    .\end{align*}

    \bigbreak \noindent \bigbreak \noindent 
    \begin{Large}
        \noindent \textbf{Question 11:}
    \end{Large}
    \bigbreak \noindent 
    \pf{Solution}{}
    \bigbreak \noindent 
    \textit{$G ^{\prime}(r)$:}
    \begin{align*}
      G ^{\prime}(r) = r^{ \frac{1}{2}} + r^{ \frac{1}{5}} \\ 
      = \frac{1}{2}r^{ ^{-\frac{1}{2}}} + \frac{1}{5}r^{ ^{-\frac{4}{5}}} \\ 
      = \frac{1}{2r^{ \frac{1}{2}}} + \frac{1}{5r^{ \frac{4}{5}}}
    .\end{align*}
    \bigbreak \noindent 
    \textit{$g ^{\prime\prime}(r)$:}
    \begin{align*}
      G ^{\prime\prime}(r) = \frac{1}{2}r^{ ^{-\frac{1}{2}}} + \frac{1}{5}r^{ ^{-\frac{4}{5}}} \\
      = - \frac{1}{4}r^{ ^{-\frac{3}{2}}} - \frac{4}{25}r^{ ^{-\frac{9}{5}}} \\ 
      = - \frac{1}{4r^{ \frac{3}{2}}} - \frac{4}{25r^{ \frac{9}{5}}}
    .\end{align*}


    \bigbreak \noindent \bigbreak \noindent 
    \begin{Large}
        \noindent \textbf{Question 12:}
    \end{Large}
    \bigbreak \noindent 
    \pf{Solution}{}
    \bigbreak \noindent 
    \textbf{a.)}
    \begin{align*}
      0.101 * 50 = 5.05
    .\end{align*}
    \bigbreak \noindent 
    \textit{So:}
    \begin{align*}
      \frac{5.05}{P}
    .\end{align*}
    \bigbreak \noindent 
    \textit{b.)}
    \bigbreak \noindent 
    \textit{$V ^{\prime}(P)$:}
    \begin{align*}
      V ^{\prime}(P) = 5.05p^{-1} \\
      = -5.05p^{-2} \\ 
      = - \frac{5.05}{p^2}
    .\end{align*}
    \textit{Plug in 50 for P:}
    \begin{align*}
      - \frac{5.05}{50^2} \\ 
      = -0.00202
    .\end{align*}

    \bigbreak \noindent \bigbreak \noindent 
    \begin{Large}
        \noindent \textbf{Question 13:}
    \end{Large}
    \bigbreak \noindent 
    \pf{Solution}{}
    \bigbreak \noindent 
    \textit{$y ^{\prime}$:}
    \begin{align*}
      y ^{\prime} = 3x^2+6x-9(1)-0 \\
      = 3x^2+6x-9
    .\end{align*}


    \bigbreak \noindent \bigbreak \noindent 
    \begin{Large}
        \noindent \textbf{Question 14:}
    \end{Large}
    \bigbreak \noindent 
    \pf{Solution}{}
    \bigbreak \noindent 

    \bigbreak \noindent \bigbreak \noindent 
    \begin{Large}
        \noindent \textbf{Question 15:}
    \end{Large}
    \bigbreak \noindent 
    \pf{Solution}{}
    \bigbreak \noindent 

\end{document}
