\documentclass{report}

\input{~/dev/latex/template/preamble.tex}
\input{~/dev/latex/template/macros.tex}

\title{\Huge{3.2 Hw Solutions}}
\author{\huge{Nathan Warner}}
\date{\huge{Feb 16, 2023}}

\pgfpagesdeclarelayout{boxed}
{
  \edef\pgfpageoptionborder{0pt}
}
{
  \pgfpagesphysicalpageoptions
  {%
    logical pages=1,%
  }
  \pgfpageslogicalpageoptions{1}
  {
    border code=\pgfsetlinewidth{1.5pt}\pgfstroke,%
    border shrink=\pgfpageoptionborder,%
    resized width=.95\pgfphysicalwidth,%
    resized height=.95\pgfphysicalheight,%
    center=\pgfpoint{.5\pgfphysicalwidth}{.5\pgfphysicalheight}%
  }%
}

\pgfpagesuselayout{boxed}

\begin{document}
    \maketitle
    \begin{Large}
        \noindent \textbf{Question 1:}
    \end{Large}
    \bigbreak \noindent 
    \pf{Solution}{}
    \bigbreak \noindent 
    \textit{If:}
    \begin{align*}
        \frac{d}{dx}[f(x) \cdot g(x)] = f(x) \frac{d}{dx}[g(x)] + g(x) \frac{d}{dx}[f(x)]
    .\end{align*}
    \bigbreak \noindent 
    \textit{And:}
    \begin{align*}
        f(x) = 5x^2+4 \longrightarrow f ^{\prime}(x) = 10x \\ 
        g(x) = 7x+9 \longrightarrow g ^{\prime}(x) = 7
    .\end{align*}
    \textit{Then:}
    \begin{align*}
        y ^{\prime} = (5x^2+4)(7) + (7x+9)(10x) \\ 
        = 105x^2+90x+28
    .\end{align*}

    \bigbreak \noindent \bigbreak \noindent 
    \begin{Large}
        \textbf{Question 2:}
    \end{Large}
    \bigbreak \noindent 
    \pf{Solution}{}
    \bigbreak \noindent 
    \textit{If:}
    \begin{align*}
        \frac{d}{dx}[f(x) \cdot g(x)] = f(x) \frac{d}{dx}[g(x)] + g(x) \frac{d}{dx}[f(x)]
    .\end{align*}
    \bigbreak \noindent 
    \textit{And:}
    \begin{align*}
        f(x) = x^4 \longrightarrow f ^{\prime}(x) = 4x^3 \\ 
        g(x) = e^x \longrightarrow g ^{\prime}(x) = e^x
   .\end{align*}
   \bigbreak \noindent 
   \textit{Then:}
   \begin{align*}
       y ^{\prime} = (x^4)(e^x) + (e^x)(4x^3) \\ 
       = x^4e^x + 4x^3e^x \\
       = x^3e^x(x+4)
   .\end{align*}

    \bigbreak \noindent \bigbreak \noindent 
    \begin{Large}
        \textbf{Question 3:}
    \end{Large}
    \bigbreak \noindent 
    \pf{Solution}{}
    \bigbreak \noindent 
    \textit{If:}
    \begin{align*}
        \frac{d}{dx}[f(x) \cdot g(x)] = f(x) \frac{d}{dx}[g(x)] + g(x) \frac{d}{dx}[f(x)]
    .\end{align*}
    \bigbreak \noindent 
    \textit{And:}
    \begin{align*}
        f(x) = (7x^2-4x) \longrightarrow f ^{\prime}(x) = (14x-4) \\
        g(x) = e^x \longrightarrow g ^{\prime}(x) = e^x
    .\end{align*}
    \bigbreak \noindent 
    \textit{Then:}
    \begin{align*}
        (7x^2-4x)(e^x) + (e^x)(14x-4)  \\ 
        = 7x^2e^x-4xe^x+14xe^x-4e^x \\ 
        = 7x^2e^x+10xe^x-4e^x \\ 
        = e^x(7x^2+10x-4)
    .\end{align*}
    \bigbreak \noindent \bigbreak \noindent 
    \begin{Large}
        \textbf{Question 4:}
    \end{Large}
    \bigbreak \noindent 
    \pf{Solution}{}
    \bigbreak \noindent 
    \textit{If:}
    \begin{align*}
        \frac{d}{dx}\bigg[ \frac{f(x)}{g(x)}\bigg] = \frac{g(x) \frac{d}{dx}[f(x)] - f(x) \frac{d}{dx}[g(x)]}{[g(x)]^2}
    .\end{align*}
    \bigbreak \noindent 
    \textit{And:}
    \begin{align*}
        f(x) = e^x \longrightarrow f ^{\prime}(x) = e^x \\ 
        g(x) = (4-e^x) \longrightarrow g ^{\prime}(x) = -e^x
    .\end{align*}
    \bigbreak \noindent 
    \textit{Then:}
    \begin{align*}
        y ^{\prime} = \frac{(4-e^x)(e^x) - (e^x)(-e^x)}{(4-e^x)^2} \\
        = \frac{4e^x - e^{2x} + e^{2x}}{(4-e^x)^2} \\ 
        = \frac{4e^x}{(4-e^x)^2}
    .\end{align*}

    \bigbreak \noindent \bigbreak \noindent 
    \begin{Large}
        \textbf{Question 5:}
    \end{Large}
    \bigbreak \noindent 
    \pf{Solution}{}
    \bigbreak \noindent 
    \begin{align*}
        f ^{\prime}(u) = 12u^3-8 \\
        h ^{\prime}(u) = 1
    .\end{align*}
    \bigbreak \noindent 
    \textit{If:}
    \begin{align*}
        \frac{d}{dx}\bigg[ \frac{f(x)}{g(x)}\bigg] = \frac{g(x) \frac{d}{dx}[f(x)] - f(x) \frac{d}{dx}[g(x)]}{[g(x)]^2}
    .\end{align*}
    \bigbreak \noindent 
    \textit{Then:}
    \begin{align*}
        G ^{\prime}(u) = \frac{(u+1)(12u^3-8)-(3u^4-8u)(1)}{(u+1)^2} \\ 
        = \frac{12u^4-8u+12u^3-8-(3u^4-8u)}{(u+1)^2} \\
        = \frac{12u^4-8u+12u^3-8-3u^4+8u}{(u+1)^2} \\ 
        = \frac{9u^4+12u^3-8}{(u+1)^2}
    .\end{align*}

    \bigbreak \noindent \bigbreak \noindent 
    \begin{Large}
        \textbf{Question 6:}
    \end{Large}
    \bigbreak \noindent 
    \pf{Solution}{}
    \bigbreak \noindent 
    \textit{If:}
    \begin{align*}
        \frac{d}{dx}[f(x) \cdot g(x)] = f(x) \frac{d}{dx}[g(x)] + g(x) \frac{d}{dx}[f(x)]
    .\end{align*}
    \bigbreak \noindent 
    \textit{And:}
    \begin{align*}
        f(x) = (4u^{-1}+4u{-2}) \\
        f ^{\prime}(x) = (-4u{-2}-8u^{-3})
    .\end{align*}
    \begin{align*}
        g(x) = (2u+2u^{-1}) \\ 
        g ^{\prime}(x) = (2-2u^{-2})
    .\end{align*}
    \bigbreak \noindent 
    \textit{Then:}
    \begin{align*}
        J ^{\prime}(u) = (4u^{-1}+4u^{-2})(2-2u^{-2}) + (2u+2u{-1})(-4u^{-2}-8u^{-3}) \\ 
        = (8u^{-1}-8u^{-3}+8u{-2}-8u^{-4}) + (-8u^{-1}-16u^{-2}-8u^{-3}16u^{-4}) \\ 
        = -8u^{-3}+8u{-2}-8u^{-4} -16u^{-2}-8u^{-3}16u^{-4} \\ 
        = -16u^{-3} -8u^{-2}-24u{-4} \\ 
        = -\frac{16}{u^3} - \frac{8}{u^2} - \frac{24}{u^4}
    .\end{align*}

    \bigbreak \noindent \bigbreak \noindent 
    \begin{Large}
        \textbf{Question 7:}
    \end{Large}
    \bigbreak \noindent 
    \pf{Solution}{}
    \bigbreak \noindent 
    In this problem we need to use both formulas, product rule in the numerator to find $f ^{\prime}(x)$. 
    And then the quotient rule once we found $f ^{\prime}(x)$.
    \bigbreak \noindent 
    \textit{So $f ^{\prime}(x)$: If $f(x) = x^7$ and $g(x) = e^x$}
    \begin{align*}
        f ^{\prime}(x) = (x^7)(e^x)+(e^x)(7x^6) \\ 
        = x^7e^x+7x^6e^x
    .\end{align*}
    \bigbreak \noindent 
    \textit{Now:} 
    \begin{align*}
        \frac{(x^7+e^x)(x^7e^x+7x^6e^x) - (x^7e^x)(7x^6e^x)}{(x^7+e^x)^2} \\ 
        = \frac{(x^{14}e^x+7x^{13}e^x+x^7e^{2x}+7x^6e^{2x}) - (7x^{13}e^x+x^7e^{2x})}{(x^7+e^x)^2} \\
        = \frac{x^{14}e^x+7x^{13}e^x+x^7e^{2x}+7x^6e^{2x} - 7x^{13}e^x-x^7e^{2x}}{(x^7+e^x)^2} \\
        = \frac{x^{14}e^x+7x^6e^{2x}}{(x^7+e^x)^2} \\
        = \frac{x^6(x^8e^x+7e^{2x})}{(x^7+e^x)^2} \\
    .\end{align*}
    
    \bigbreak \noindent \bigbreak \noindent 
    \begin{Large}
        \textbf{Question 8:}
    \end{Large}
    \bigbreak \noindent 
    \pf{Solution}{}
    \bigbreak \noindent 




    \bigbreak \noindent \bigbreak \noindent 
    \begin{Large}
        \textbf{Question 9:}
    \end{Large}
    \bigbreak \noindent 
    \pf{Solution}{}
    \bigbreak \noindent 

    \bigbreak \noindent \bigbreak \noindent 
    \begin{Large}
        \textbf{Question 10:}
    \end{Large}
    \bigbreak \noindent 
    \pf{Solution}{}
    \bigbreak \noindent 
    

    \bigbreak \noindent \bigbreak \noindent 
    \begin{Large}
        \textbf{Question 11:}
    \end{Large}
    \bigbreak \noindent 
    \pf{Solution}{}
    \bigbreak \noindent 

    \bigbreak \noindent \bigbreak \noindent 
    \begin{Large}
        \textbf{Question 12:}
    \end{Large}
    \bigbreak \noindent 
    \pf{Solution}{}
    \bigbreak \noindent 

    \bigbreak \noindent \bigbreak \noindent 
    \begin{Large}
        \textbf{Question 13:}
    \end{Large}
    \bigbreak \noindent 
    \pf{Solution}{}
    \bigbreak \noindent 
    
\end{document}
